program_logic/saved_prop.v
@@ -8,9 +8,19 @@ Notation savedPropG Λ Σ :=
 Instance inGF_savedPropG `{inGF Λ Σ agreeF} : savedPropG Λ Σ.
 Proof. apply: inGF_inG. Qed.
 
-Definition saved_prop_own `{savedPropG Λ Σ}
+Definition saved_prop_own_def `{savedPropG Λ Σ}
     (γ : gname) (P : iPropG Λ Σ) : iPropG Λ Σ :=
   own γ (to_agree (Next (iProp_unfold P))).
+(* Perform sealing. *)
+Module Type SavedPropOwnSig.
+  Parameter saved_prop_own : ∀ `{savedPropG Λ Σ} (γ : gname) (P : iPropG Λ Σ),
+    iPropG Λ Σ.
+  Axiom saved_prop_own_def : @saved_prop_own = @saved_prop_own_def.
+End SavedPropOwnSig.
+Module Export SavedPropOwn : SavedPropOwnSig.
+  Definition saved_prop_own := @saved_prop_own_def.
+  Definition saved_prop_own_def := Logic.eq_refl (@saved_prop_own).
+End SavedPropOwn. 
 Instance: Params (@saved_prop_own) 4.
 
 Section saved_prop.
@@ -20,20 +30,20 @@ Section saved_prop.
 
   Global Instance saved_prop_always_stable γ P :
     AlwaysStable (saved_prop_own γ P).
-  Proof. by rewrite /AlwaysStable /saved_prop_own always_own. Qed.
+  Proof. by rewrite /AlwaysStable saved_prop_own_def always_own. Qed.
 
   Lemma saved_prop_alloc_strong N P (G : gset gname) :
     True ⊑ pvs N N (∃ γ, ■ (γ ∉ G) ∧ saved_prop_own γ P).
-  Proof. by apply own_alloc_strong. Qed.
+  Proof. by rewrite saved_prop_own_def; apply own_alloc_strong. Qed.
 
   Lemma saved_prop_alloc N P :
     True ⊑ pvs N N (∃ γ, saved_prop_own γ P).
-  Proof. by apply own_alloc. Qed.
+  Proof. by rewrite saved_prop_own_def; apply own_alloc. Qed.
 
   Lemma saved_prop_agree γ P Q :
     (saved_prop_own γ P ★ saved_prop_own γ Q) ⊑ ▷ (P ≡ Q).
   Proof.
-    rewrite /saved_prop_own -own_op own_valid agree_validI.
+    rewrite saved_prop_own_def -own_op own_valid agree_validI.
     rewrite agree_equivI later_equivI /=; apply later_mono.
     rewrite -{2}(iProp_fold_unfold P) -{2}(iProp_fold_unfold Q).
     apply (eq_rewrite (iProp_unfold P) (iProp_unfold Q) (λ Q' : iPreProp Λ _,
